Rearranging lemmas

src/simple-proof/proof/Binding.v
@@ -12,6 +12,66 @@ Require Import LibLN.
 Require Import Coq.Program.Equality.
 Require Import Definitions.
 
+(** * Substitution Definitions *)
+
+(** Substitution on variables: [a[u/z]] (substituting [z] with [u] in [a]). *)
+Definition subst_avar (z: var) (u: var) (a: avar) : avar :=
+  match a with
+  | avar_b i => avar_b i
+  | avar_f x => (avar_f (If x = z then u else x))
+  end.
+
+(** Substitution on types and declarations: [T[u/z]] and [D[u/z]]. *)
+Fixpoint subst_typ (z: var) (u: var) (T: typ) { struct T } : typ :=
+  match T with
+  | typ_top        => typ_top
+  | typ_bot        => typ_bot
+  | typ_rcd D      => typ_rcd (subst_dec z u D)
+  | typ_and T1 T2  => typ_and (subst_typ z u T1) (subst_typ z u T2)
+  | typ_sel x L    => typ_sel (subst_avar z u x) L
+  | typ_bnd T      => typ_bnd (subst_typ z u T)
+  | typ_all T U    => typ_all (subst_typ z u T) (subst_typ z u U)
+  end
+with subst_dec (z: var) (u: var) (D: dec) { struct D } : dec :=
+  match D with
+  | dec_typ L T U => dec_typ L (subst_typ z u T) (subst_typ z u U)
+  | dec_trm L U => dec_trm L (subst_typ z u U)
+  end.
+
+(** Substitution on terms, values, and definitions:
+    [t[u/z]], [v[u/z]], [d[u/z]]. *)
+Fixpoint subst_trm (z: var) (u: var) (t: trm) : trm :=
+  match t with
+  | trm_var x        => trm_var (subst_avar z u x)
+  | trm_val v        => trm_val (subst_val z u v)
+  | trm_sel x1 L     => trm_sel (subst_avar z u x1) L
+  | trm_app x1 x2    => trm_app (subst_avar z u x1) (subst_avar z u x2)
+  | trm_let t1 t2    => trm_let (subst_trm z u t1) (subst_trm z u t2)
+  end
+with subst_val (z: var) (u: var) (v: val) : val :=
+  match v with
+  | val_new T ds     => val_new (subst_typ z u T) (subst_defs z u ds)
+  | val_lambda T t   => val_lambda (subst_typ z u T) (subst_trm z u t)
+  end
+with subst_def (z: var) (u: var) (d: def) : def :=
+  match d with
+  | def_typ L T => def_typ L (subst_typ z u T)
+  | def_trm L t => def_trm L (subst_trm z u t)
+  end
+with subst_defs (z: var) (u: var) (ds: defs) : defs :=
+  match ds with
+  | defs_nil => defs_nil
+  | defs_cons rest d => defs_cons (subst_defs z u rest) (subst_def z u d)
+  end.
+
+(** Substitution on the types of a typing environment: [G[u/z]]. *)
+Definition subst_ctx (z: var) (u: var) (G: ctx) : ctx :=
+  map (subst_typ z u) G.
+
+(** Substitution on the values of an evaluation context: [e[y/x]]. *)
+Definition subst_env x y e := map (subst_val x y) e.
+
+
 (** * Lemmas About Opening *)
 
 Ltac avar_solve :=
@@ -636,4 +696,295 @@ Lemma binds_fv_ec_vals : forall x y v e,
 Proof.
   intros. unfold fv_ec_vals in H0.
   eapply fv_in_values_binds; eauto.
+Qed.
+
+(** * Lemmas about variable substitution *)
+
+(** [e(b) = v]            #<br>#
+    [――――――――――――――――――]  #<br>#
+    [e[y/x](b) = v[y/x]]  *)
+Lemma binds_subst_env : forall x y b v e,
+    binds b v e -> binds b (subst_val x y v) (subst_env x y e).
+Proof.
+  introv. gen x y b v. induction e using env_ind; intros.
+  - destruct (binds_empty_inv H).
+  - apply binds_push_inv in H.
+    destruct_all; subst; unfold subst_env; rewrite map_push.
+    + auto.
+    + apply binds_push_neq; auto.
+Qed.
+
+(** Substitution preserves local closure. *)
+
+(** - for variables *)
+Lemma lc_at_subst_avar : forall v x y k,
+    lc_at_var k v <-> lc_at_var k (subst_avar x y v).
+Proof.
+  intros.
+  split; intros;
+    try solve [inversion H; simpls; auto].
+  destruct v; auto.
+Qed.
+
+(** - for types and declarations *)
+Lemma lc_at_subst_typ_dec : forall k,
+  (forall T, lc_at_typ k T -> forall x y, lc_at_typ k (subst_typ x y T)) /\
+  (forall D, lc_at_dec k D -> forall x y, lc_at_dec k (subst_dec x y D)).
+Proof.
+  apply lc_at_typ_mutind; intros; simpls; auto.
+  constructor. apply lc_at_subst_avar. trivial.
+Qed.
+
+(** - for terms, values, and definitions *)
+Lemma lc_at_subst_trm_val_def_defs : forall k,
+    (forall t, lc_at_trm k t -> forall x y, lc_at_trm k (subst_trm x y t)) /\
+    (forall v, lc_at_val k v -> forall x y, lc_at_val k (subst_val x y v)) /\
+    (forall d, lc_at_def k d -> forall x y, lc_at_def k (subst_def x y d)) /\
+    (forall ds, lc_at_defs k ds -> forall x y, lc_at_defs k (subst_defs x y ds)).
+Proof.
+  apply lc_at_mutind; intros; simpls; auto;
+    repeat constructor;
+    try solve [apply lc_at_subst_avar; trivial];
+    try apply lc_at_subst_typ_dec; trivial.
+Qed.
+
+(** The following [subst_fresh_XYZ] lemmas state that if [x] is not free
+    in a symbol [Y], then [Y[z/x] = Y]. *)
+
+(** Fresh substitution
+    - in variables *)
+Lemma subst_fresh_avar: forall x y,
+  (forall a: avar, x \notin fv_avar a -> subst_avar x y a = a).
+Proof.
+  intros. destruct* a. simpl. case_var*. simpls. notin_false.
+Qed.
+
+(** - in types and declarations *)
+Lemma subst_fresh_typ_dec: forall x y,
+  (forall T : typ , x \notin fv_typ  T  -> subst_typ  x y T  = T ) /\
+  (forall D : dec , x \notin fv_dec  D  -> subst_dec  x y D  = D ).
+Proof.
+  intros x y. apply typ_mutind; intros; simpls; f_equal*.
+  apply* subst_fresh_avar.
+Qed.
+
+Definition subst_fresh_typ(x y: var) := proj1 (subst_fresh_typ_dec x y).
+
+(** - in terms, values, and definitions *)
+Lemma subst_fresh_trm_val_def_defs: forall x y,
+  (forall t : trm , x \notin fv_trm  t  -> subst_trm  x y t  = t ) /\
+  (forall v : val , x \notin fv_val  v  -> subst_val  x y v  = v ) /\
+  (forall d : def , x \notin fv_def  d  -> subst_def  x y d  = d ) /\
+  (forall ds: defs, x \notin fv_defs ds -> subst_defs x y ds = ds).
+Proof.
+  intros x y. apply trm_mutind; intros; simpls; f_equal*;
+    (apply* subst_fresh_avar || apply* subst_fresh_typ_dec).
+Qed.
+
+(** [x \notin fv(G, z: T)]                   #<br>#
+    [x \notin fv(T)]                         #<br>#
+    [―――――――――――――――――――――――――――――――――――――] #<br>#
+    [x \notin fv(T)] and [x \notin fv(G)] *)
+Lemma invert_fv_ctx_types_push: forall x z T G,
+  x \notin fv_ctx_types (G & z ~ T) -> x \notin fv_typ T /\ x \notin (fv_ctx_types G).
+Proof.
+  introv H. rewrite fv_ctx_types_push_eq in H.
+  apply~ notin_union.
+Qed.
+
+(** [x \notin fv(G)]         #<br>#
+    [――――――――――――――――――]    #<br>#
+    [G[y/x] = G]    *)
+Lemma subst_fresh_ctx: forall x y G,
+  x \notin fv_ctx_types G -> subst_ctx x y G = G.
+Proof.
+  intros x y.
+  apply (env_ind (fun G => x \notin fv_ctx_types G -> subst_ctx x y G = G)).
+  + intro N. unfold subst_ctx. apply map_empty.
+  + intros G z T IH N.
+    apply invert_fv_ctx_types_push in N. destruct N as [N1 N2].
+    unfold subst_ctx in *. rewrite map_push.
+    rewrite (IH N2).
+    rewrite ((proj1 (subst_fresh_typ_dec _ _)) _ N1).
+    reflexivity.
+Qed.
+
+(** Definition of substitution on named variables: #<br>#
+    [z[y/x] := if z == x then y else z], where [z] is a named variable. *)
+Definition subst_fvar(x y z: var): var := If z = x then y else z.
+
+(** The following lemmas state that substitution commutes with opening:
+    for a symbol [Z], #<br>#
+    [(Z^a)[y/x] = (Z[y/x])^(a[y/x])]. *)
+
+(** Substitution commutes with opening
+    - variables *)
+Lemma subst_open_commut_avar: forall x y u,
+  (forall a: avar, forall n: Datatypes.nat,
+    subst_avar x y (open_rec_avar n u a)
+    = open_rec_avar n (subst_fvar x y u) (subst_avar  x y a)).
+Proof.
+  intros. unfold subst_fvar, subst_avar, open_avar, open_rec_avar. destruct a.
+  + repeat case_if; auto.
+  + case_var*.
+Qed.
+
+(** - types and declarations *)
+Lemma subst_open_commut_typ_dec: forall x y u,
+  (forall t : typ, forall n: nat,
+     subst_typ x y (open_rec_typ n u t)
+     = open_rec_typ n (subst_fvar x y u) (subst_typ x y t)) /\
+  (forall D : dec, forall n: nat,
+     subst_dec x y (open_rec_dec n u D)
+     = open_rec_dec n (subst_fvar x y u) (subst_dec x y D)).
+Proof.
+  intros. apply typ_mutind; intros; simpl; f_equal*.
+  apply subst_open_commut_avar.
+Qed.
+
+(** - types only *)
+Lemma subst_open_commut_typ: forall x y u T,
+  subst_typ x y (open_typ u T) = open_typ (subst_fvar x y u) (subst_typ x y T).
+Proof.
+  intros. apply subst_open_commut_typ_dec.
+Qed.
+
+(** - terms, values, definitions, and list of definitions *)
+Lemma subst_open_commut_trm_val_def_defs: forall x y u,
+  (forall t : trm, forall n: Datatypes.nat,
+     subst_trm x y (open_rec_trm n u t)
+     = open_rec_trm n (subst_fvar x y u) (subst_trm x y t)) /\
+  (forall v : val, forall n: Datatypes.nat,
+     subst_val x y (open_rec_val n u v)
+     = open_rec_val n (subst_fvar x y u) (subst_val x y v)) /\
+  (forall d : def , forall n: Datatypes.nat,
+     subst_def x y (open_rec_def n u d)
+     = open_rec_def n (subst_fvar x y u) (subst_def x y d)) /\
+  (forall ds: defs, forall n: Datatypes.nat,
+     subst_defs x y (open_rec_defs n u ds)
+     = open_rec_defs n (subst_fvar x y u) (subst_defs x y ds)).
+Proof.
+  intros. apply trm_mutind; intros; simpl; f_equal~;
+    (apply subst_open_commut_avar || apply subst_open_commut_typ_dec).
+Qed.
+
+(** - terms only *)
+Lemma subst_open_commut_trm: forall x y u t,
+    subst_trm x y (open_trm u t)
+    = open_trm (subst_fvar x y u) (subst_trm x y t).
+Proof.
+  intros. apply subst_open_commut_trm_val_def_defs.
+Qed.
+
+(** - definitions only *)
+Lemma subst_open_commut_defs: forall x y u ds,
+    subst_defs x y (open_defs u ds)
+    = open_defs (subst_fvar x y u) (subst_defs x y ds).
+Proof.
+  intros. apply subst_open_commut_trm_val_def_defs.
+Qed.
+
+(** The following lemmas state that opening a symbol with a variable [y]
+    is the same as opening the symbol with another variable [x] and
+    substituting [x] with [y]: #<br>#
+    [Z^y = (Z^x)[y/x]] *)
+
+(** Substitution after opening
+    - terms *)
+Lemma subst_intro_trm: forall x u t, x \notin (fv_trm t) ->
+  open_trm u t = subst_trm x u (open_trm x t).
+Proof.
+  introv Fr. unfold open_trm. rewrite subst_open_commut_trm.
+  destruct (@subst_fresh_trm_val_def_defs x u) as [Q _]. rewrite~ (Q t).
+  unfold subst_fvar. case_var~.
+Qed.
+
+(** - definitions *)
+Lemma subst_intro_defs: forall x u ds, x \notin (fv_defs ds) ->
+  open_defs u ds = subst_defs x u (open_defs x ds).
+Proof.
+  introv Fr. unfold open_trm. rewrite subst_open_commut_defs.
+  destruct (@subst_fresh_trm_val_def_defs x u) as [_ [_ [_ Q]]]. rewrite~ (Q ds).
+  unfold subst_fvar. case_var~.
+Qed.
+
+(** - types *)
+Lemma subst_intro_typ: forall x u T, x \notin (fv_typ T) ->
+  open_typ u T = subst_typ x u (open_typ x T).
+Proof.
+  introv Fr. unfold open_typ. rewrite subst_open_commut_typ.
+  destruct (@subst_fresh_typ_dec x u) as [Q _]. rewrite~ (Q T).
+  unfold subst_fvar. case_var~.
+Qed.
+
+Ltac subst_open_fresh :=
+  repeat match goal with
+    | [ |- context [ open_typ ?z (subst_typ ?x ?y ?T) ] ] =>
+        replace (open_typ z (subst_typ x y T)) with (open_typ (subst_fvar x y z) (subst_typ x y T))
+          by (unfold subst_fvar; rewrite~ If_r);
+        rewrite_all <- subst_open_commut_typ
+    | [ |- context [ open_defs ?z (subst_defs ?x ?y ?ds) ] ] =>
+        replace (open_defs z (subst_defs x y ds)) with (open_defs (subst_fvar x y z) (subst_defs x y ds))
+          by (unfold subst_fvar; rewrite~ If_r);
+        rewrite_all <- subst_open_commut_defs
+     | [ |- context [ open_trm ?z (subst_trm ?x ?y ?t) ] ] =>
+        replace (open_trm z (subst_trm x y t)) with (open_trm (subst_fvar x y z) (subst_trm x y t))
+          by (unfold subst_fvar; rewrite~ If_r);
+        rewrite_all <- subst_open_commut_trm
+    end.
+
+(** Substitution preserves labels of definitions: [label(d) = label(d[y/x])] *)
+Lemma subst_label_of_def: forall x y d,
+  label_of_def d = label_of_def (subst_def x y d).
+Proof.
+  intros. destruct d; reflexivity.
+Qed.
+
+(** [l \notin labels(ds)]     #<br>#
+    [――――――――――――――――――――――] #<br>#
+    [l \notin labels(ds[y/x]] *)
+Lemma subst_defs_hasnt: forall x y l ds,
+  defs_hasnt ds l ->
+  defs_hasnt (subst_defs x y ds) l.
+Proof.
+  intros x y l ds. unfold defs_hasnt. induction ds; introv Eq.
+  - reflexivity.
+  - unfold get_def. simpl. rewrite <- subst_label_of_def.
+    simpl in Eq. case_if~.
+Qed.
+
+(** [z <> x]                             #<br>#
+    [ds^z = ...{a = t}...]              #<br>#
+    [――――――――――――――――――――――――――――――――]  #<br>#
+    [(ds[y/x])^z = ...{a = t[y/x]}...]  *)
+Lemma open_subst_defs : forall x y z a ds t,
+    z <> x ->
+    defs_has (open_defs z ds) (def_trm a t) ->
+    defs_has (open_defs z (subst_defs x y ds)) (def_trm a (subst_trm x y t)).
+Proof.
+  introv. gen x y z a t. induction ds; intros.
+  - inversion H0.
+  - unfold open_defs, defs_has in *; simpls. case_if.
+    + destruct d; simpls; case_if; auto.
+      inversions H0.
+      rewrite subst_open_commut_trm. unfold subst_fvar.
+      case_if. auto.
+    + case_if; apply IHds; destruct d; auto; contradiction.
+Qed.
+
+(** [y <> x]                             #<br>#
+    [ds^x = ...{a = t}...]              #<br>#
+    [――――――――――――――――――――――――――――――――]  #<br>#
+    [(ds[y/x])^y = ...{a = t[y/x]}...]  *)
+Lemma open_subst_defs2 : forall x y a ds t,
+    y <> x ->
+    defs_has (open_defs x ds) (def_trm a t) ->
+    defs_has (open_defs y (subst_defs x y ds)) (def_trm a (subst_trm x y t)).
+Proof.
+  introv. gen x y a t. induction ds; intros.
+  - inversion H0.
+  - unfold open_defs, defs_has in *.
+    simpls; case_if; destruct d; simpls; case_if; auto.
+    subst; inversion H0.
+    rewrite subst_open_commut_trm. unfold subst_fvar. case_if; auto.
 Qed.
